WebAssembly/Wasm_Interpreter_Printing.thy
@@ -7,15 +7,33 @@ definition "run_invoke = run_invoke_v (2^63) 300"
 (* host *)
 
 axiomatization
-  Abs_host :: "((s \<times> v list) \<Rightarrow> (s \<times> v list) option) \<Rightarrow> host" and
-  Rep_host :: "host \<Rightarrow> ((s \<times> v list) \<Rightarrow> (s \<times> v list) option)"
+  Abs_host_func :: "((s \<times> v list) \<Rightarrow> (s \<times> v list) option) \<Rightarrow> host_func" and
+  Rep_host_func :: "host_func \<Rightarrow> ((s \<times> v list) \<Rightarrow> (s \<times> v list) option)"
 where
-  host_is[code abstype]:
-    "Abs_host (Rep_host h) = h"
+  host_func_is[code abstype]:
+    "Abs_host_func (Rep_host_func h) = h"
 and
   host_apply_impl_def[code] :
-    "host_apply_impl s tf h vs = ((Rep_host h) (s,vs))"
+    "host_func_apply_impl s tf h vs = ((Rep_host_func h) (s,vs))"
 
+
+code_printing
+  type_constructor host_ref \<rightharpoonup> (OCaml) "int32"
+  
+
+(*  type_constructor i32 \<rightharpoonup> (OCaml) "I32Wrapper.t" *)
+(*| type_constructor i64 \<rightharpoonup> (OCaml) "I64Wrapper.t" *)
+(*
+axiomatization
+  Abs_host_ref :: "integer \<Rightarrow> host_ref" and
+  Rep_host_ref :: "host_ref \<Rightarrow> integer"
+where
+  host_ref_is[code abstype]:
+    "Abs_host_ref (Rep_host_ref hr) = hr"
+and
+  host_ref_is2[code abstype]:
+    "Rep_host_ref (Abs_host_ref n) = n"
+*)
 (* memory *)
 
 (*
